src/LocalBlockchain.v
@@ -1,0 +1,108 @@
+From Coq Require Import ZArith.
+From SmartContracts Require Import Blockchain.
+From SmartContracts Require Import Oak.
+From SmartContracts Require Import Monads.
+From Containers Require Import Maps.
+From Coq Require Import List.
+
+Import ListNotations.
+(* Note that [ ] or nil is needed for the empty list
+   in this file as [] parses an empty map *)
+
+Local Record ContractInstance :=
+  {
+    inst_state_ty : OakType;
+    inst_msg_ty : OakType;
+    inst_state : interp_type inst_state_ty;
+    inst_receive : ContractCallContext -> interp_type inst_state_ty ->
+                   option (interp_type inst_msg_ty) -> ChainAction;
+  }.
+
+Local Record ChainUpdate :=
+  {
+    upd_block : Block;
+    (* Contracts that had their states updated and the new state *)
+    upd_contracts : Map[Address, ContractInstance];
+    (* Contracts deployed in this block *)
+    upd_deployments : Map[Address, ContractDeployment];
+    (* All transactions caused by update, including internal txs
+       (due to contract execution) *)
+    upd_txs : list Tx;
+  }.
+
+Inductive LocalChain :=
+  {
+    lc_updates : list ChainUpdate;
+  }.
+
+Definition genesis_block : Block :=
+  {| block_header := {| block_number := 0; |};
+     block_txs := nil |}.
+
+Definition initial_chain : LocalChain :=
+  {| lc_updates :=
+       [{| upd_block := genesis_block;
+           upd_contracts := []%map;
+           upd_deployments := []%map;
+           upd_txs := nil |}]
+  |}.
+
+Definition lc_chain_at (lc : LocalChain) (bid : BlockId) : option LocalChain :=
+  let is_old u := u.(upd_block).(block_header).(block_number) <=? bid in
+  let new_updates := filter is_old lc.(lc_updates) in
+  match new_updates with
+  | hd :: tl => if hd.(upd_block).(block_header).(block_number) =? bid
+                then Some {| lc_updates := new_updates |}
+                else None
+  | nil => None
+  end.
+
+Definition lc_block_at (lc : LocalChain) (bid : BlockId) : option Block :=
+  let blocks := map upd_block lc.(lc_updates) in
+  find (fun b => b.(block_header).(block_number) =? bid) blocks.
+
+Definition lc_head_block (lc : LocalChain) : Block :=
+  match lc.(lc_updates) with
+  | hd :: _ => hd.(upd_block)
+  | nil => genesis_block
+  end.
+
+Definition lc_incoming_txs (lc : LocalChain) (addr : Address) : list Tx :=
+  let all_txs := flat_map (fun u => u.(upd_block).(block_txs)) lc.(lc_updates) in
+  let is_inc tx := (tx.(tx_to) =? addr)%address in
+  filter is_inc all_txs.
+
+Definition lc_outgoing_txs (lc : LocalChain) (addr : Address) : list Tx :=
+  let all_txs := flat_map (fun u => u.(upd_block).(block_txs)) lc.(lc_updates) in
+  let is_out tx := (tx.(tx_from) =? addr)%address in
+  filter is_out all_txs.
+
+Local Definition find_first {A : Type} (f : ChainUpdate -> option A) (lc : LocalChain)
+  : option A :=
+  let opts := map f lc.(lc_updates) in
+  let is_some o := match o with | Some _ => true | None => false end in
+  match filter is_some opts with
+  | hd :: _ => hd
+  | _ => None
+  end.
+
+Definition lc_contract_deployment (lc : LocalChain) (addr : Address)
+  : option ContractDeployment :=
+  find_first (fun u => u.(upd_deployments)[addr]%map) lc.
+  
+Definition lc_contract_state (lc : LocalChain) (addr : Address)
+  : option OakValue :=
+  let get_state_oak_value u :=
+      do c <- u.(upd_contracts)[addr]%map;
+      Some (build_oak_value c.(inst_state_ty) c.(inst_state)) in
+  find_first get_state_oak_value lc.
+
+Definition local_chain_impl : ChainInterface :=
+  {| ifc_chain_type := LocalChain;
+     ifc_chain_at := lc_chain_at;
+     ifc_head_block := lc_head_block;
+     ifc_incoming_txs := lc_incoming_txs;
+     ifc_outgoing_txs := lc_outgoing_txs;
+     ifc_contract_deployment := lc_contract_deployment;
+     ifc_contract_state := lc_contract_state;
+  |}.
